\subsection*{Aufgabe 33}
Gegeben für $i, n \in \NN_0$ mit $i < n$ Bernstein Polynome $B_i^n \in \RR[x]$ mit
\begin{align}
  B_i^n(x) = \binom{n}{i} x^i(1 - x)^{n-i}
\end{align}
und für eine Funktion $f: [0,1] \rightarrow \RR$
\begin{align}
  (B_n f)(x) = \sum_{i = 0}^n f\left(\frac{i}{n}\right) B_i^n(x) =
  \sum_{i = 0}^n f\left(\frac{i}{n}\right) \binom{n}{i} x^i(1 - x)^{n-i}
\end{align}
Berechne $(B_n f)(x)$ für $f_0(x) = x^0, f_1(x) = x^1, f_2(x) = x^2$.

\begin{align*}
  f_0(x) &= \sum_{i = 0}^n 1 \cdot \binom{n}{i} x^i(1 - x)^{n-i}
    \; \overset{\text{Binom. Lehrsatz}}{=} \; \left( x + (1 -x) \right)^n = 1^n = 1 \quad \Box\\
  f_1(x) &= \sum_{i = 0}^n \frac{i}{n} \; \frac{n!}{i! (n-i)!} x^i(1 - x)^{n-i} =
    \sum_{i = 1}^n \frac{i}{n} \; \frac{n!}{i! (n-i)!} x^i(1 - x)^{n-i} \\
    & = \sum_{i = 1}^n \frac{(n-1)!}{(i-1)! (n-i)!} \cdot x \cdot x^{(i-1)}(1 - x)^{n-i}
    \quad \text{mit $k = i - 1$} \\
    & = x  \cdot \sum_{k = 0}^{n-1} \frac{n!}{k! (n-k)!} x^k(1 - x)^{n-k}
    = x \cdot \left( x + (1 -x) \right)^{n-1} = x \cdot 1^{n-1} = x  \quad \Box\\
  f_2(x) &= \sum_{i = 0}^n \left(\frac{i}{n}\right)^2 \frac{n!}{i! (n-i)!} x^i(1 - x)^{n-i} =
  \text{TODO} = \frac{x}{n} + \frac{n-1}{n} x^2  \quad \Box
\end{align*}

